Coq/Payoff/CutPayoffN.v
@@ -1,0 +1,227 @@
+(* Some (unfinished) attempts to generalize proof about cutPayoff
+   to n step contract reduction *)
+Require Import Tactics.
+Require Import ILSyntax.
+Require Import ILSemantics.
+Require Import Denotational.
+Require Import Syntax.
+Require Import Utils.
+Require Import Horizon.
+Require Import Misc.
+Require Import Reduction.
+Require Import Typing.
+Require Import Templates.
+Require Import ILTranslation.
+Require Import CutPayoff.
+
+Require Import List.
+Require Import ZArith.
+Require Import Arith.
+Require Import FunctionalExtensionality.
+Require Import Coq.Program.Equality.
+
+Import Nat.
+
+(* N step contract reduction *)
+Inductive RedN : nat -> Contr -> EnvP -> ExtEnvP -> Contr ->  Prop :=
+    red_refl c envp extp : RedN O c envp extp c
+  | red_step c c' c'' n envp extp tr : RedN n c envp extp c'' -> Red c'' envp extp c' tr ->
+                             RedN (S n) c envp extp c'.
+
+Hint Constructors RedN Red.
+
+Example RedN_ex1 : forall envp extp cur p1 p2,
+                     RedN 3 (Translate (Tnum 2) (Transfer cur p1 p2)) envp extp Zero.
+Proof.
+  intros. econstructor. econstructor. econstructor. econstructor. econstructor.
+  reflexivity. reflexivity. econstructor.
+  reflexivity. reflexivity.
+  econstructor. econstructor. econstructor. reflexivity.
+Qed.
+
+Lemma adv_disc_0 d:
+  adv_disc 0 d = d.
+Proof.
+  unfold adv_disc. simpl. apply functional_extensionality. reflexivity.
+Qed.
+
+Lemma fromContr_Red_exists c c' t0 tr extp envp il_e:
+  fromContr c t0 = Some il_e ->
+  Red c envp extp c' tr ->
+  exists il_e', fromContr c' t0 = Some il_e'.
+Proof.
+Admitted.
+
+Lemma fromContr_RedN_exists c c' n t0 extp envp il_e:
+  fromContr c t0 = Some il_e ->
+  RedN n c envp extp c' ->
+  exists il_e', fromContr c' t0 = Some il_e'.
+Proof.
+  Admitted.
+
+Lemma fromContr_ILsem_Red_exists c c' t0 tr extp envp il_e il_e' disc p1 p2 extIL tenv r:
+  fromContr c t0 = Some il_e ->
+  Red c envp extp c' tr ->
+  fromContr c' t0 = Some il_e' ->
+  IL[|il_e|]extIL tenv 0 0 disc p1 p2 = Some (ILRVal r) ->
+  exists r', IL[|cutPayoff il_e'|](adv_ext 1 extIL) tenv 0 1 disc p1 p2 = Some (ILRVal r').
+Proof.
+  Admitted.
+
+Lemma fromContr_ILsem_RedN_exists c c' n t0 extp envp il_e il_e' disc p1 p2 extIL tenv r:
+  fromContr c t0 = Some il_e ->
+  RedN n c envp extp c' ->
+  fromContr c' t0 = Some il_e' ->
+  IL[|cutPayoff il_e|]extIL tenv 0 (S n) disc p1 p2 = Some (ILRVal r) ->
+  exists r', IL[|cutPayoff il_e'|](adv_ext (Z.of_nat n) extIL) tenv 0 1 disc p1 p2 = Some (ILRVal r').
+Proof.
+Admitted.
+
+Definition cutPayoff_sound c n :=
+  forall envC extC (il_e : ILExpr) (extIL : ExtEnv' ILVal) (envP : EnvP) (extP : ExtEnvP)
+         (v' : ILVal) m n0 p1 p2 curr v trace (disc : nat -> R ) tenv,
+  (forall a a', Asset.eqb a a' = true) ->
+  (forall l t, fromVal (extC l t) = extIL l t) ->
+  IsClosedCT c ->
+  fromContr c (ILTexpr (Tnum n0)) = Some il_e ->
+  C[|Translate (Tnum n0) c|] envC extC tenv = Some trace ->
+  m + n = horizon c tenv ->
+  sum_list (map (fun t => (disc t * trace t p1 p2 curr)%R)
+                (seq (n+n0) m)) = v ->
+  IL[|cutPayoff il_e|] extIL tenv 0 (n+n0) disc p1 p2 = Some v'->
+  fromVal (RVal v) = v'.
+
+Hint Resolve delay_empty_trace.
+
+Lemma cutPayoff_sound_base c : cutPayoff_sound c 0.
+Proof.
+  unfold cutPayoff_sound. intros.
+  eapply Contr_translation_sound with (tenv:=tenv) (envC:=envC) (disc:=disc); eauto;
+  try rewrite plus_0_r in *; try rewrite plus_0_l in *; subst; try eassumption; try reflexivity.
+  erewrite ILexpr_eq_cutPayoff_at_n with (c:=c) (t0:=(ILTexpr (Tnum n0))); try eassumption. reflexivity.
+  simpl. apply not_true_is_false. intro. apply Nat.ltb_lt in H4. omega.
+Qed.
+
+Lemma cp_Scale_inversion c n e :
+  cutPayoff_sound (Scale e c) n -> cutPayoff_sound c n.
+Proof.
+Admitted.
+
+Lemma cp_Translate_inversion c t0 n :
+  cutPayoff_sound (Translate t0 c) n -> cutPayoff_sound c n.
+Proof.
+Admitted.
+
+Lemma sum_delay_n':
+  forall (n n0 : nat) (tr : Trace) (p1 p2 : Party) (curr : Asset) (f : nat -> R) (t0 n1 : nat),
+  sum_list (map (fun t : nat => (f t * delay_trace (n0 + n) tr t p1 p2 curr)%R) (seq (t0 + n0) n1)) =
+  sum_list (map (fun t : nat => (f (n0 + t)%nat * delay_trace n tr t p1 p2 curr)%R) (seq t0 n1)).
+Proof.
+  Admitted.
+
+Lemma cp_sound_translate_1 c n :
+  cutPayoff_sound c n -> cutPayoff_sound (Translate (Tnum 1) c) (1 + n).
+Proof.
+  unfold cutPayoff_sound.
+  intros until tenv; intros A Xeq TC CC Cs Hor Sm ILs.
+  inversion TC.
+  eapply H with (m:=m) (n0:= S n0);eauto.
+  + rewrite Equivalence.transl_iter in Cs. replace (S n0) with (n0 + 1) by ring.
+    apply Cs.
+  + simpl in *. destruct (horizon c tenv). destruct m;simpl in *;tryfalse.
+    simpl in Hor. omega.
+  + simpl in *. replace (n + S n0) with (S (n + n0)) by ring. eapply Sm.
+  + replace (n + S n0) with (S (n + n0)) by ring. eapply ILs.
+Qed.
+
+Fixpoint transl_one_iter (n : nat) (c : Contr) :=
+  match n with
+  | O => Translate (Tnum 1) c
+  | S n' => Translate (Tnum 1) (transl_one_iter n' c)
+  end.
+
+(* I think, this property is required for the n-step proof *)
+Lemma cp_summ c n :
+  forall envC extC (il_e : ILExpr) (extIL : ExtEnv' ILVal) (envP : EnvP) (extP : ExtEnvP)
+         (v' : ILVal) m n0 p1 p2 curr v v'' trace (disc : nat -> R ) tenv,
+    (forall a a', Asset.eqb a a' = true) ->
+    (forall l t, fromVal (extC l t) = extIL l t) ->
+    IsClosedCT c ->
+    fromContr c (ILTexpr (Tnum n0)) = Some il_e ->
+    C[|Translate (Tnum n0) c|] envC extC tenv = Some trace ->
+    m + n = horizon c tenv ->
+    sum_list (map (fun t => (disc t * trace t p1 p2 curr)%R)
+                  (seq (n+n0) m)) = v ->
+    IL[|cutPayoff il_e|] extIL tenv 0 (n+n0) disc p1 p2 = Some v' ->
+    fromVal (RVal v) = v' ->
+    IL[|cutPayoff il_e|] extIL tenv 0 (1+n+n0) disc p1 p2 = Some (ILRVal v'') ->
+    v' = ILRVal (trace (n+n0)%nat p1 p2 curr + v'')%R.
+Proof.
+  Admitted.
+  
+Lemma cutPayoff_sound_step c n :
+      cutPayoff_sound c n -> cutPayoff_sound c (1 + n).
+Proof.
+  generalize dependent n.
+  induction c; intros until tenv; intros A Xeq TC CC Cs Hor S ILs.
+  - (* zero *)
+    simpl in *. some_inv. subst. simpl in *.
+    unfold compose,bind,pure in *. some_inv. rewrite sum_of_map_empty_trace; auto.
+  - (* let *)
+    simpl in *. option_inv_auto.
+  - (* transf *)
+    intros. simpl in *. option_inv_auto. unfold compose in *. some_inv.
+    remember (Party.eqb p p0) as b0.
+    destruct b0.
+    + simpl in *. assert (Hmeq0 : m=0) by omega. subst. simpl. some_inv. reflexivity.
+    + simpl in *. assert (Hmeq0 : m=0) by omega. assert (Hneq0 : n = 0 ) by omega. subst. simpl.
+      rewrite plus_0_l in *.
+      assert (Hlt_true : (n0 <? S n0) = true). apply Nat.ltb_lt. omega.
+      rewrite Hlt_true in *. some_inv. reflexivity.
+  - (* scale *)
+    intros. simpl in *. option_inv_auto. some_inv. subst. simpl in *. option_inv_auto.
+    destruct_vals. some_inv. subst. rewrite delay_trace_scale.
+    unfold scale_trace, compose, scale_trans.
+    rewrite summ_list_common_factor. rewrite <- fromVal_RVal_eq. apply fromVal_RVal_f_eq.
+    + erewrite <- cutPayoff_eq_compiled_expr in H5; try eassumption.
+      eapply Exp_translation_sound with (t0':=0) (envT:=tenv) (envC:=envC);
+        try (simpl in *; some_inv; subst); try eassumption.
+      rewrite Z.add_0_r. assumption.
+    + inversion TC. apply cp_Scale_inversion in H.
+      eapply IHc with (envC:=envC); eauto. simpl. autounfold.
+      rewrite H2. reflexivity.
+  - (* translate *)
+    intros.
+    simpl in *. option_inv_auto. rewrite delay_trace_swap.
+    inversion TC. subst. simpl in *.
+    rename n1 into t0.
+    simpl in *.
+    rewrite adv_ext_iter in H2.
+    replace (Z.of_nat n0 + Z.of_nat t0)%Z with (Z.of_nat (t0 + n0)) in *.
+    rewrite delay_trace_iter.
+    destruct t0.
+    * apply cp_Translate_inversion in H.
+      rewrite add_0_r. simpl in *. rewrite <- fromVal_RVal_eq.
+      eapply IHc with (envC:=envC);eauto.
+      simpl. autounfold. rewrite H2. reflexivity.
+      destruct (horizon c tenv);destruct m;simpl in *;tryfalse;auto.
+    * apply cp_Translate_inversion in H.
+      destruct t0. unfold cutPayoff_sound in H.
+      ** eapply H with (m:=m) (n0:= S n0);eauto.
+         *** simpl. autounfold.
+             (* replace (Z.of_nat n0 + 1)%Z with (1 + Z.of_nat n0)%Z by ring. *)
+             (* rewrite succ_of_nat with (t:=0%Z). simpl.          *)
+             simpl in H2. rewrite H2. autounfold. reflexivity.
+         *** simpl in *. destruct (horizon c tenv). destruct m;simpl in *; tryfalse.
+             simpl in *. omega.
+         *** simpl. replace (n0 +1) with (S n0) by ring.
+             replace (n + S n0) with (S (n + n0)) by ring. reflexivity.
+         *** replace (n + S n0) with (S (n + n0)) by ring. assumption.
+Admitted.
+
+Theorem cutPayoff_sound_n_steps c n: cutPayoff_sound c n.
+Proof.
+  induction n.
+  - apply cutPayoff_sound_base.
+  - apply cutPayoff_sound_step. apply IHn.
+Qed.
